Add cabal project for extracted code with custom Setup.hs

Setup.hs
@@ -1,0 +1,24 @@
+-- editorconfig-checker-disable-file
+{-# LANGUAGE OverloadedStrings #-}
+import Data.Functor
+import Distribution.Simple
+import Distribution.Simple.Setup
+import Distribution.Types.HookedBuildInfo
+import Distribution.Types.LocalBuildInfo
+import Distribution.Types.PackageDescription
+import Turtle
+
+main :: IO ()
+main = defaultMainWithHooks userhooks
+
+userhooks :: UserHooks
+userhooks = simpleUserHooks {
+      postConf = \_ _ _ _ -> runMake
+    , preBuild = \_ _ -> runMake >> pure emptyHookedBuildInfo
+    }
+
+runMake :: IO ()
+runMake = procs "make" [] empty
+
+-- runAgda :: IO ()
+-- runAgda = procs "agda" ["--compile", "--ghc-dont-call-ghc", "--local-interfaces", "src/Main.lagda"] empty
